

$$y = ax^3 + bx^2 + cx. \quad y' = 3ax^2 + 2bx + c. \quad c = y' - 3ax^2 - 2bx. \quad \text{Подставив, получим}$$

$$y = ax^3 + bx^2 + xy' - 3ax^3 - 2bx^2. \quad \begin{cases} y = -2ax^3 - bx^2 + xy' \\ y' = -6ax^2 - 2bx + y' + xy'' \end{cases}$$

$$2y = -4ax^3 - 2bx \cdot x + 2xy' = -4ax^3 + 2xy' - x(xy'' - 6ax^2) = 2ax^3 + 2xy' - x^2y''.$$

$$\begin{cases} 2y = 2ax^3 + 2xy' - x^2y'' \\ 2y' = 6ax^2 + 2y' + 2xy'' - 2xy'' - x^2y''' \end{cases} \cdot 6a = y'''. \quad 6y = x^3y''' + 6xy' - 3x^2y'' = 0.$$

Итак, $x^3y''' - 3x^2y'' + 6xy' - 6y = 0$.